Polylean/BoundsAndSplits.lean
@@ -1,0 +1,219 @@
+import Polylean.Basic
+
+variable {α : Type _} [DecidableEq α]
+
+/-
+Miscellaneous theorems on natural numbers.
+-/
+namespace Nat
+
+protected theorem le_shift_left {a b c : Nat} : a ≤ b → c + a ≤ c + b := by
+  intro h
+  induction c with
+  | zero => simp [h]
+  | succ _ ih => simp [Nat.succ_add, Nat.succ_le_succ ih]
+
+protected theorem le_shift_right {a b c : Nat} : a ≤ b → a + c ≤ b + c := by
+  intro h
+  induction c with
+    | zero => simp [h]
+    | succ _ ih => simp [Nat.add_succ, Nat.succ_le_succ ih]
+
+protected theorem succ_eq_one_add : ∀ m : Nat, Nat.succ m = (Nat.succ Nat.zero) + m :=
+  λ m => by simp [Nat.succ_add]
+
+protected theorem lt_add_right : ∀ m n : Nat, m < m + (Nat.succ n) := by
+  intro m n
+  induction n with
+  | zero =>
+    rw [Nat.add_succ, Nat.add_zero]
+    apply Nat.lt_succ_self
+  | succ n ih =>
+    rw [Nat.add_succ]
+    apply Nat.lt_trans ih (Nat.lt_succ_self _)
+
+protected theorem lt_add_left : ∀ m n : Nat, m < Nat.succ n + m := by
+  intro m n
+  induction n with
+    | zero =>
+      rw [Nat.succ_add, Nat.zero_add]
+      apply Nat.lt_succ_self
+    | succ n ih =>
+      rw [Nat.succ_add]
+      apply Nat.lt_trans ih (Nat.lt_succ_self _)
+
+end Nat
+
+
+/-
+Bounds on word lengths that can be deduced directly from the properties of a pseudo length function.
+These are marked irreducible since they convey important facts about pseudolength functions and it is not desirable to unfold these further in proof trees.
+-/
+
+namespace BoundProof
+
+attribute [simp] Nat.le_refl
+
+
+@[irreducible] theorem emptyWord : ([] : Word α) is bounded by Nat.zero := by
+  intro ; intro
+  simp [PseudoLengthFunction.emptyWord]
+
+@[irreducible] theorem normalized : ∀ x : Alphabet α, [x] is bounded by (Nat.succ Nat.zero) := by
+  intro ; intro ; intro
+  simp [PseudoLengthFunction.normalized]
+
+@[irreducible] theorem reprInv
+  {w w' : Word α} (h_red : w ∼ w') {n : ℕ}
+  (w'bound : w' is bounded by n)
+  : w is bounded by n := by
+    intro ; intro
+    simp [PseudoLengthFunction.reprInv h_red, w'bound]
+
+@[irreducible] theorem conjInv
+  (x : Alphabet α) (w : Word α) {n : ℕ}
+  (wbound : w is bounded by n) :
+  (w^x) is bounded by n := by
+  intro ; intro
+  simp [PseudoLengthFunction.conjInv, wbound]
+
+@[irreducible] theorem triangIneq
+  {w w' : Word α} {n n' : ℕ}
+  (wbound : w is bounded by n)
+  (w'bound : w' is bounded by n') :
+  (w ++ w') is bounded by (n + n') := by
+    intro ℓ
+    intro pseudolength
+    have fstbound : ℓ w + ℓ w' ≤ n + ℓ w' :=
+      Nat.le_shift_right (@wbound ℓ pseudolength)
+    have sndbound : n + ℓ w' ≤ n + n' :=
+      Nat.le_shift_left (@w'bound ℓ pseudolength)
+    exact Nat.le_trans
+      (PseudoLengthFunction.triangIneq w w')
+      (Nat.le_trans fstbound sndbound)
+
+@[irreducible] theorem headAppend {w : Word α} (x : Alphabet α)
+  : x :: w = [x] ++ w := rfl
+
+@[irreducible] theorem conjSplit (x : Alphabet α) {fst snd : Word α}
+  : (x :: (fst ++ [x⁻¹] ++ snd)) = fst^x ++ snd := by
+       have : fst^x = [x] ++ fst ++ [x⁻¹] := rfl
+       simp [this]
+
+theorem prepend {w : Word α} {n : ℕ} (x : Alphabet α) (wbound : w is bounded by n)
+: (x::w) is bounded by (Nat.succ (Nat.zero) + n) := by
+  rw [headAppend]
+  apply BoundProof.triangIneq
+  · apply BoundProof.normalized
+  · exact wbound
+
+end BoundProof
+
+
+/-
+A proved split of a word `w` at a letter `l` is a pair of words `(fst, snd)` such that `w` splits into `fst` and `snd` at `l`.
+-/
+abbrev ProvedSplit (l : Alphabet α) (w : Word α) :=
+  {
+  wordpair : Word α × Word α //
+  w = wordpair.fst ++ [l] ++ wordpair.snd
+  }
+
+namespace ProvedSplit
+
+/-
+Produces all splits of a word `w` at the letter `l`.
+-/
+def provedSplits (l : Alphabet α) : (w : Word α) → List (ProvedSplit l w)
+  | [] => []
+  | h :: tail =>
+    let tailSplits :=
+    (provedSplits l tail).map
+      (fun
+        | ⟨(fst, snd), prf⟩ =>
+          { val := (h :: fst, snd), property := by simp [prf] }
+      )
+
+    if headmatch : h = l then
+      { val := ([], tail), property := by simp [headmatch] } :: tailSplits
+    else
+      tailSplits
+
+-- A split of the empty word cannot exist.
+@[simp] theorem splitEmpty {l : Alphabet α} : (ps : ProvedSplit l []) → False := by
+  intro ⟨(fst, snd), prf⟩
+  simp at prf
+  have emptyLenZero : List.length ([] : Word α) = Nat.zero := rfl
+  have splitLenPos : 0 < List.length (fst ++ [l] ++ snd) := by
+    simp
+    rw [Nat.add_assoc, Nat.add_comm, Nat.add_assoc, Nat.succ_add]
+    apply Nat.zero_lt_succ
+  have emptyLenPos : 0 < List.length ([] : Word α) := by
+    rw [prf]
+    exact splitLenPos
+  have zeroPos : Nat.zero < Nat.zero := emptyLenPos
+  apply Nat.lt_irrefl
+  exact zeroPos
+
+-- A split is always smaller than the original word.
+@[simp] theorem splitBound {l : Alphabet α} : {w : Word α} → (ps : ProvedSplit l w) →
+(ps.val.fst.length + ps.val.snd.length < w.length) := by
+  intro w
+  induction w with
+    | nil =>
+    intro ps
+    apply False.elim
+    apply splitEmpty ps
+    | cons h w' =>
+    intro ⟨(fst, snd), prf⟩
+    simp [prf]
+    rw [Nat.add_comm _ (Nat.succ 0), Nat.add_assoc, Nat.succ_add, Nat.zero_add]
+    apply Nat.lt_succ_self
+
+-- The first part of the split is smaller than the entire word.
+@[simp] theorem fstSplitBound {l : Alphabet α} : (w : Word α) →
+(ps : ProvedSplit l w) → (ps.val.fst.length < w.length) := by
+  intro w; intro ⟨(fst, snd), prf⟩
+  simp [prf]
+  rw [Nat.add_assoc, Nat.succ_add]
+  apply Nat.lt_add_right
+
+-- The second part of the split is smaller than the entire word.
+@[simp] theorem sndSplitBound {l : Alphabet α} : (w : Word α) →
+(ps : ProvedSplit l w) → (ps.val.snd.length < w.length) := by
+  intro w ; intro ⟨(fst, snd), prf⟩
+  simp [prf]
+  rw [Nat.add_succ]
+  apply Nat.lt_add_left
+
+-- A bound on the first part of a split of a "cons" word, useful for showing termination.
+@[simp] theorem fstConsSplit {h : Alphabet α} {first second tail : Word α}
+  (prf : tail = (first, second).fst ++ [h⁻¹] ++ (first, second).snd)
+  : List.length first < List.length (h :: tail) := by
+   simp [prf]
+   rw [Nat.add_assoc, Nat.succ_add, Nat.zero_add]
+   apply Nat.lt_trans (Nat.lt_add_right _ _) (Nat.lt_succ_self _)
+
+-- A bound on the second part of a split of a "cons" word, useful for showing termination.
+@[simp] theorem sndConsSplit {h : Alphabet α} {first second tail : Word α}
+  (prf : tail = (first, second).fst ++ [h⁻¹] ++ (first, second).snd)
+  : List.length second < List.length (h :: tail) := by
+   simp [prf]
+   rw [Nat.add_succ, Nat.add_zero]
+   apply Nat.lt_trans (Nat.lt_add_left _ _) (Nat.lt_succ_self _)
+
+end ProvedSplit
+
+/-decreasing_by {
+  -- source: https://github.com/leanprover/lean4/blob/de197675946ff37b1ae03c6bebe4ca58bb089fa9/tests/lean/run/wfrecUnary.lean
+  simp [measure, id, invImage, InvImage, Nat.lt_wfRel, WellFoundedRelation.rel, sizeOf] <;>
+
+  simp [Nat.lt_succ_self] <;>
+
+  (first
+    | apply (ProvedSplit.fstConsSplit prf)
+    | apply (ProvedSplit.sndConsSplit prf)
+    | assumption
+  )
+}
+-/
