Polylean/WatsonCrickLength.lean
@@ -1,0 +1,129 @@
+import Polylean.BoundsAndSplits
+
+/-
+A non-crossing match is inductively defined to be one of
+- the empty word
+- a letter of the alphabet attached to the front of a non-crossing match
+- a conjugate of a non-crossing match appended to the front of a non-crossing match
+
+Example:
+
+  .---------.
+    .--.
+α β α α⁻¹ β β⁻¹  ↦   α :: (matching β (matching α [] (β :: [])) [])
+-/
+inductive MatchWord (α : Type _) [DecidableEq α]
+  | nil : MatchWord α
+  | cons : Alphabet α → MatchWord α → MatchWord α
+  | matching : Alphabet α → MatchWord α → MatchWord α → MatchWord α
+  deriving Repr --, DecidableEq
+
+
+namespace MatchWord
+
+variable {α : Type _} [DecidableEq α]
+
+/-
+The number of un-matched letters in a matching.
+-/
+@[reducible, simp] def unmatchedCount : MatchWord α → ℕ
+  | nil => 0
+  | cons l w => 1 + unmatchedCount w
+  | matching _ w w' => unmatchedCount w + unmatchedCount w'
+
+/-
+Converts a non-crossing match word to the corresponding usual word.
+-/
+@[reducible, simp] def toWord : MatchWord α → Word α
+  | nil => []
+  | cons l w => l :: (toWord w)
+  | matching l w w' => (toWord w)^l ++ (toWord w')
+
+
+/-
+Defining a "matching" corresponding to a word.
+-/
+@[reducible] def isMatching (m : MatchWord α) (w : Word α) := m.toWord = w
+
+infix:100 " is a matching of " => MatchWord.isMatching
+
+abbrev Matching (w : Word α) := {m : MatchWord α // m is a matching of w}
+
+
+/-
+A total order on the matchings of a word in terms of the "energy" (the number of unmatched letters).
+-/
+instance {w : Word α} : LE (Matching w) :=
+ ⟨λ m m' => unmatchedCount m.val ≤ unmatchedCount m'.val⟩
+
+instance {w : Word α} : ∀ m m' : Matching w, Decidable (m ≤ m') := by
+  intro ; intro
+  simp [LE.le]; exact inferInstance
+
+
+/-
+The empty matching cannot correspond to a non-empty word.
+-/
+theorem consNeEmptyMatch (l : Alphabet α) (w : Word α) : ¬(nil is a matching of (l :: w)) := by
+  intro h_match ; simp [isMatching] at h_match
+
+/-
+If `m` is a matching of a word `w`, the length of `w` under any pseudo-length function is
+bounded by the "energy" of `m` (the number of unmatched letters).
+
+This theorem is crucial for proving the maximality of the Watson-Crick length.
+-/
+theorem unmatchedCountBound (m : MatchWord α)
+  : (m.toWord is bounded by m.unmatchedCount) := by
+  induction m with
+    | nil =>
+      intro ; intro
+      simp [PseudoLengthFunction.emptyWord]
+    | cons =>
+      intro ; intro
+      apply BoundProof.prepend
+      assumption
+    | matching =>
+      intro ; intro
+      apply BoundProof.triangIneq
+      · apply BoundProof.conjInv ; assumption
+      · assumption
+
+/-
+Takes a word `w` as input and returns a maximal matching
+(a matching with the lowest number of unmatched letters) of the word.
+-/
+def maxMatch : (w : Word α) → Matching w
+  | List.nil => ⟨MatchWord.nil, rfl⟩  -- the trivial case of the empty word
+  | List.cons l w' =>
+
+    -- the case where the first letter is unmatched
+    let base : Matching (l :: w') :=
+      let ⟨w'Match, w'Prf⟩ := maxMatch w'
+      ⟨MatchWord.cons l w'Match, by simp [w'Prf]⟩
+
+    -- the case where the first letter is matched
+    let splits : List (Matching (l :: w')) :=
+    (ProvedSplit.provedSplits l⁻¹ w').map (λ ⟨⟨fst, snd⟩, prf⟩ =>
+          -- proof that the length of the word decreases, required for showing termination
+          have : fst.length < (l :: w').length := ProvedSplit.fstConsSplit prf
+          let ⟨fstMatch, fstPrf⟩ := maxMatch fst -- a maximal matching of the first part of the split
+
+          -- proof that the length of the word decreases, required for showing termination
+          have : snd.length < (l :: w').length := ProvedSplit.sndConsSplit prf
+          let ⟨sndMatch, sndPrf⟩ := maxMatch snd -- a maximal matching of the second part of the split
+
+          {
+            -- creates a matching involving the first letter of the word
+            val := (MatchWord.matching l fstMatch sndMatch),
+            property := by
+             rw [prf, BoundProof.conjSplit, ← fstPrf, ← sndPrf]
+          }
+      )
+
+    -- the best matching of the ones above, i.e., the one with the least unmatched letters ("energy")
+    splits.foldl min base
+
+termination_by _ w => List.length w -- this function terminates since the length of the input list decreases on each recursive call
+
+namespace MatchWord
